Vibe coding the other direction. Admit free

rupicola/io/LogRelTargetSource.CompatibilityLemmas.fst
@@ -1027,6 +1027,59 @@ let helper_equiv_oprod_if_steps_pre (g:typ_env) (e:closed_exp) (h:history) (lt:l
   (forall (lt:local_trace h). t ⫃ (h++lt, (fs_e2 fsG), e2)) /\
   (forall (lt:local_trace h). t ⫃ (h++lt, (fs_e3 fsG), e3))
 
+#push-options "--z3rlimit 15 --split_queries always"
+let helper_equiv_oprod_if_steps (h:history) (lt:local_trace h) (t:qType)
+  (fs_e1:fs_prod qBool) (fs_e2 fs_e3:fs_prod t) (fs_r:fs_val t)
+  (e1 e2 e3:closed_exp) :
+  Lemma
+    (requires fs_beh (fs_prod_bind fs_e1 (fun x -> fs_prod_if_val x fs_e2 fs_e3)) h lt fs_r /\
+              qBool ⫃ (h, fs_e1, e1) /\
+              (forall (lt':local_trace h). t ⫃ (h++lt', fs_e2, e2)) /\
+              (forall (lt':local_trace h). t ⫃ (h++lt', fs_e3, e3)))
+    (ensures exists e'. t ∈ (h++lt, fs_r, e') /\ e_beh (EIf e1 e2 e3) e' h lt) =
+  let fs_k : fs_val qBool -> fs_prod t = fun x -> fs_prod_if_val x fs_e2 fs_e3 in
+  assert (fs_prod_bind fs_e1 fs_k == io_bind fs_e1 fs_k) by (norm [delta_only [`%fs_prod_bind]]; trefl ());
+  destruct_fs_beh fs_e1 fs_k h lt fs_r;
+  eliminate exists (lt1:local_trace h) (lt2:local_trace (h++lt1)) (fs_b:fs_val qBool).
+    lt == (lt1@lt2) /\ fs_beh fs_e1 h lt1 fs_b /\ fs_beh (fs_k fs_b) (h++lt1) lt2 fs_r
+    returns exists e'. t ∈ (h++lt, fs_r, e') /\ e_beh (EIf e1 e2 e3) e' h lt with _. begin
+  // From qBool ⫃ (h, fs_e1, e1), get the boolean value expression
+  eliminate forall (lt':local_trace h) (fs_r':get_Type qBool). fs_beh fs_e1 h lt' fs_r' ==> exists e1'. qBool ∈ (h++lt', fs_r', e1') /\ e_beh e1 e1' h lt' with lt1 fs_b;
+  eliminate exists e1'. qBool ∈ (h++lt1, fs_b, e1') /\ e_beh e1 e1' h lt1
+    returns exists e'. t ∈ (h++lt, fs_r, e') /\ e_beh (EIf e1 e2 e3) e' h lt with _. begin
+  lem_values_are_values qBool (h++lt1) fs_b e1';
+  lem_value_is_irred e1';
+  trans_history h lt1 lt2;
+  if fs_b then begin
+    assert (e1' == ETrue);
+    assert (fs_beh fs_e2 (h++lt1) lt2 fs_r);
+    // From forall lt'. t ⫃ (h++lt', fs_e2, e2), specialize with lt1
+    assert (t ⫃ (h++lt1, fs_e2, e2));
+    eliminate forall (lt'':local_trace (h++lt1)) (fs_r':get_Type t).
+      fs_beh fs_e2 (h++lt1) lt'' fs_r' ==> exists e'. t ∈ ((h++lt1)++lt'', fs_r', e') /\ e_beh e2 e' (h++lt1) lt'' with lt2 fs_r;
+    eliminate exists e'. t ∈ ((h++lt1)++lt2, fs_r, e') /\ e_beh e2 e' (h++lt1) lt2
+      returns exists e'. t ∈ (h++lt, fs_r, e') /\ e_beh (EIf e1 e2 e3) e' h lt with _. begin
+    FStar.Squash.bind_squash #(steps e1 e1' h lt1) () (fun sts_e1 ->
+    FStar.Squash.bind_squash #(steps e2 e' (h++lt1) lt2) () (fun sts_branch ->
+    construct_steps_eif e1 ETrue e2 e3 e' h lt1 lt2 sts_e1 sts_branch))
+    end
+  end else begin
+    assert (e1' == EFalse);
+    assert (fs_beh fs_e3 (h++lt1) lt2 fs_r);
+    assert (t ⫃ (h++lt1, fs_e3, e3));
+    eliminate forall (lt'':local_trace (h++lt1)) (fs_r':get_Type t).
+      fs_beh fs_e3 (h++lt1) lt'' fs_r' ==> exists e'. t ∈ ((h++lt1)++lt'', fs_r', e') /\ e_beh e3 e' (h++lt1) lt'' with lt2 fs_r;
+    eliminate exists e'. t ∈ ((h++lt1)++lt2, fs_r, e') /\ e_beh e3 e' (h++lt1) lt2
+      returns exists e'. t ∈ (h++lt, fs_r, e') /\ e_beh (EIf e1 e2 e3) e' h lt with _. begin
+    FStar.Squash.bind_squash #(steps e1 e1' h lt1) () (fun sts_e1 ->
+    FStar.Squash.bind_squash #(steps e3 e' (h++lt1) lt2) () (fun sts_branch ->
+    construct_steps_eif e1 EFalse e2 e3 e' h lt1 lt2 sts_e1 sts_branch))
+    end
+  end
+  end
+  end
+#pop-options
+
 #push-options "--split_queries always"
 let equiv_oprod_if #g
   (#t:qType)
@@ -1050,9 +1103,10 @@ let equiv_oprod_if #g
       assert (gsubst s (EIf e1 e2 e3) == e);
       let EIf e1 e2 e3 = e in
       introduce fsG `(≍) h` s ==> t ⫃ (h, fs_e, e) with _. begin
+        lem_shift_type_value_environments h fsG s;
         introduce forall lt (fs_r:fs_val t). fs_beh fs_e h lt fs_r ==> exists e'. t ∈ (h++lt, fs_r, e') /\ e_beh e e' h lt with begin
           introduce fs_beh fs_e h lt fs_r ==> exists e'. t ∈ (h++lt, fs_r, e') /\ e_beh e e' h lt with _. begin
-            admit ()
+            helper_equiv_oprod_if_steps h lt t fs_e1' fs_e2' fs_e3' fs_r e1 e2 e3
           end
         end
       end
@@ -1068,18 +1122,88 @@ let equiv_oprod_var g (x:var{Some? (g x)}) : Lemma (fs_oprod_var g x ⊑ EVar x)
   equiv_oval_var g x;
   equiv_oprod_return (fs_oval_var g x) (EVar x)
 
-let equiv_oprod_app_steps_pre' (e e':closed_exp) (h:history) (lt:local_trace h) (a b:qType) (fs_x':(fs_val (a ^->!@ b)) -> fs_prod b) (fs_f:fs_prod (a ^->!@ b)) (fs_e':fs_prod b) (f x:exp) =
-  (fs_e' == io_bind fs_f fs_x') /\
-  (e == EApp f x) /\
-  (e_beh e e' h lt) /\
-  ((a ^->!@ b) ⫃ (h, fs_f, f))
+#push-options "--z3rlimit 15 --split_queries always"
+let helper_equiv_oprod_app_steps (h:history) (lt:local_trace h) (a b:qType)
+  (fs_f':fs_prod (a ^->!@ b)) (fs_x':fs_prod a) (fs_r:fs_val b)
+  (f x:closed_exp) :
+  Lemma
+    (requires fs_beh (fs_prod_bind fs_f' (fun f' -> fs_prod_bind fs_x' (fun x' -> f' x'))) h lt fs_r /\
+              (a ^->!@ b) ⫃ (h, fs_f', f) /\
+              (forall (lt':local_trace h). a ⫃ (h++lt', fs_x', x)))
+    (ensures exists e'. b ∈ (h++lt, fs_r, e') /\ e_beh (EApp f x) e' h lt) =
+  let fs_outer_k : fs_val (a ^->!@ b) -> fs_prod b = fun f' -> fs_prod_bind fs_x' (fun x' -> f' x') in
+  assert (fs_prod_bind fs_f' fs_outer_k == io_bind fs_f' fs_outer_k) by (norm [delta_only [`%fs_prod_bind]]; trefl ());
+  destruct_fs_beh fs_f' fs_outer_k h lt fs_r;
+  eliminate exists (lt1:local_trace h) (lt2:local_trace (h++lt1)) (fs_r_f:fs_val (a ^->!@ b)).
+    lt == (lt1@lt2) /\ fs_beh fs_f' h lt1 fs_r_f /\ fs_beh (fs_outer_k fs_r_f) (h++lt1) lt2 fs_r
+    returns exists e'. b ∈ (h++lt, fs_r, e') /\ e_beh (EApp f x) e' h lt with _. begin
+  // From (a ^->!@ b) ⫃ (h, fs_f', f), get the function value
+  eliminate forall (lt':local_trace h) (fs_r':get_Type (a ^->!@ b)). fs_beh fs_f' h lt' fs_r' ==> exists e'. (a ^->!@ b) ∈ (h++lt', fs_r', e') /\ e_beh f e' h lt' with lt1 fs_r_f;
+  eliminate exists f'. (a ^->!@ b) ∈ (h++lt1, fs_r_f, f') /\ e_beh f f' h lt1
+    returns exists e'. b ∈ (h++lt, fs_r, e') /\ e_beh (EApp f x) e' h lt with _. begin
+  let ELam f1 = f' in
+  // Decompose the inner bind: fs_prod_bind fs_x' (fun x' -> fs_r_f x') at h++lt1
+  assert (fs_prod_bind fs_x' (fun x' -> fs_r_f x') == io_bind fs_x' (fun x' -> fs_r_f x')) by (norm [delta_only [`%fs_prod_bind]]; trefl ());
+  destruct_fs_beh fs_x' (fun x' -> fs_r_f x') (h++lt1) lt2 fs_r;
+  eliminate exists (lt2a:local_trace (h++lt1)) (lt2b:local_trace ((h++lt1)++lt2a)) (fs_r_x:fs_val a).
+    lt2 == (lt2a@lt2b) /\ fs_beh fs_x' (h++lt1) lt2a fs_r_x /\ fs_beh (fs_r_f fs_r_x) ((h++lt1)++lt2a) lt2b fs_r
+    returns exists e'. b ∈ (h++lt, fs_r, e') /\ e_beh (EApp f x) e' h lt with _. begin
+  // From a ⫃ (h++lt1, fs_x', x), get the argument value
+  assert (a ⫃ (h++lt1, fs_x', x));
+  eliminate forall (lt':local_trace (h++lt1)) (fs_r':get_Type a). fs_beh fs_x' (h++lt1) lt' fs_r' ==> exists e'. a ∈ ((h++lt1)++lt', fs_r', e') /\ e_beh x e' (h++lt1) lt' with lt2a fs_r_x;
+  eliminate exists x'. a ∈ ((h++lt1)++lt2a, fs_r_x, x') /\ e_beh x x' (h++lt1) lt2a
+    returns exists e'. b ∈ (h++lt, fs_r, e') /\ e_beh (EApp f x) e' h lt with _. begin
+  // Unfold IO arrow and get application result
+  unfold_member_of_io_arrow a b fs_r_f f1 (h++lt1);
+  lem_values_are_values a ((h++lt1)++lt2a) fs_r_x x';
+  eliminate forall (v:value) (fs_v:fs_val a) (lt_v:local_trace (h++lt1)).
+    a ∈ ((h++lt1)++lt_v, fs_v, v) ==> b ⫃ ((h++lt1)++lt_v, fs_r_f fs_v, subst_beta v f1) with x' fs_r_x lt2a;
+  // From b ⫃ ((h++lt1)++lt2a, fs_r_f fs_r_x, subst_beta x' f1)
+  eliminate forall (lt':local_trace ((h++lt1)++lt2a)) (fs_r':get_Type b).
+    fs_beh (fs_r_f fs_r_x) ((h++lt1)++lt2a) lt' fs_r' ==> exists e'. b ∈ (((h++lt1)++lt2a)++lt', fs_r', e') /\ e_beh (subst_beta x' f1) e' ((h++lt1)++lt2a) lt' with lt2b fs_r;
+  eliminate exists e'. b ∈ (((h++lt1)++lt2a)++lt2b, fs_r, e') /\ e_beh (subst_beta x' f1) e' ((h++lt1)++lt2a) lt2b
+    returns exists e'. b ∈ (h++lt, fs_r, e') /\ e_beh (EApp f x) e' h lt with _. begin
+  // Construct steps: EApp f x -->* e'
+  FStar.Squash.bind_squash #(steps f (ELam f1) h lt1) () (fun sts_f ->
+  FStar.Squash.bind_squash #(steps x x' (h++lt1) lt2a) () (fun sts_x ->
+  FStar.Squash.bind_squash #(steps (subst_beta x' f1) e' ((h++lt1)++lt2a) lt2b) () (fun sts_body ->
+  construct_steps_eapp f f1 x x' e' h lt1 lt2a lt2b sts_f sts_x sts_body;
+  trans_history (h++lt1) lt2a lt2b;
+  trans_history h lt1 (lt2a@lt2b))))
+  end
+  end
+  end
+  end
+  end
+#pop-options
 
 let equiv_oprod_app #g (#a #b:qType) (fs_f:fs_oprod g (a ^->!@ b)) (fs_x:fs_oprod g a) (f x:exp)
   : Lemma
     (requires fs_f ⊑ f /\ fs_x ⊑ x)
     (ensures fs_oprod_app fs_f fs_x ⊑ EApp f x) =
   lem_fv_in_env_app g f x;
-  admit ()
+  introduce forall b' (s:gsub g b') fsG h. fsG `(≍) h` s ==> b ⫃ (h, fs_oprod_app fs_f fs_x fsG, gsubst s (EApp f x)) with begin
+    introduce _ ==> _ with _. begin
+      let fs_f' : fs_prod (a ^->!@ b) = fs_f fsG in
+      let fs_x' : fs_prod a = fs_x fsG in
+      let fs_e = fs_prod_bind fs_f' (fun f' -> fs_prod_bind fs_x' (fun x' -> f' x')) in
+      assert (fs_e == fs_oprod_app fs_f fs_x fsG) by (
+        norm [delta_only [`%fs_oprod_app;`%fs_oprod_bind';`%fs_oprod_bind;`%fs_oprod_app_oval_oval]];
+        l_to_r [`lem_hd_stack;`tail_stack_inverse];
+        trefl ());
+      let e = EApp (gsubst s f) (gsubst s x) in
+      assert (gsubst s (EApp f x) == e);
+      let EApp f x = e in
+      introduce fsG `(≍) h` s ==> b ⫃ (h, fs_e, e) with _. begin
+        lem_shift_type_value_environments h fsG s;
+        introduce forall lt (fs_r:fs_val b). fs_beh fs_e h lt fs_r ==> exists e'. b ∈ (h++lt, fs_r, e') /\ e_beh e e' h lt with begin
+          introduce fs_beh fs_e h lt fs_r ==> exists e'. b ∈ (h++lt, fs_r, e') /\ e_beh e e' h lt with _. begin
+            helper_equiv_oprod_app_steps h lt a b fs_f' fs_x' fs_r f x
+          end
+        end
+      end
+    end
+  end
 
 let equiv_oprod_lambda #g (#t1:qType) (#t2:qType)
   (fs_body:fs_oprod (extend t1 g) t2)
@@ -1091,19 +1215,426 @@ let equiv_oprod_lambda #g (#t1:qType) (#t2:qType)
   equiv_oval_lambda_oprod #g #t1 #t2 fs_body body;
   equiv_oprod_return (fs_oval_lambda_oprod fs_body) (ELam body)
 
-let equiv_oprod_inl #g (t1 t2:qType) (fs_e:fs_oprod g t1) (e:exp)
-  : Lemma
-    (requires fs_e ⊑ e)
-    (ensures fs_oprod_fmap #g #t1 #(t1 ^+ t2) fs_e Inl ⊑ (EInl e))
-  = admit ()
+(** ---- Helpers for fmap-based lemmas (inl, inr, fst, snd) ---- **)
 
-let equiv_oprod_inr #g (t1 t2:qType) (fs_e:fs_oprod g t2) (e:exp)
-  : Lemma
-    (requires fs_e ⊑ e)
-    (ensures fs_oprod_fmap #g #t2 #(t1 ^+ t2) fs_e Inr ⊑ (EInr e))
-  =
-  admit ()
+#push-options "--z3rlimit 15"
+let helper_equiv_oprod_fmap_inl_steps (h:history) (lt:local_trace h) (t1 t2:qType)
+  (fs_e':fs_prod t1) (fs_r:fs_val (t1 ^+ t2)) (e:closed_exp) :
+  Lemma
+    (requires fs_beh (fs_prod_bind fs_e' (fun v -> return (Inl #(fs_val t1) #(fs_val t2) v))) h lt fs_r /\
+              t1 ⫃ (h, fs_e', e))
+    (ensures exists e'. (t1 ^+ t2) ∈ (h++lt, fs_r, e') /\ e_beh (EInl e) e' h lt) =
+  let fs_k : fs_val t1 -> fs_prod (t1 ^+ t2) = fun v -> return (Inl #(fs_val t1) #(fs_val t2) v) in
+  assert (fs_prod_bind fs_e' fs_k == io_bind fs_e' fs_k) by (norm [delta_only [`%fs_prod_bind]]; trefl ());
+  destruct_fs_beh fs_e' fs_k h lt fs_r;
+  eliminate exists (lt1:local_trace h) (lt2:local_trace (h++lt1)) (fs_v:fs_val t1).
+    lt == (lt1@lt2) /\ fs_beh fs_e' h lt1 fs_v /\ fs_beh (return (Inl #(fs_val t1) #(fs_val t2) fs_v)) (h++lt1) lt2 fs_r
+    returns exists e'. (t1 ^+ t2) ∈ (h++lt, fs_r, e') /\ e_beh (EInl e) e' h lt with _. begin
+  let val_ = Inl #(fs_val t1) #(fs_val t2) fs_v in
+  theta_monad_morphism_ret val_;
+  let p : hist_post (h++lt1) (get_Type (t1 ^+ t2)) = fun lt' r' -> lt' == [] /\ r' == val_ in
+  assert (hist_return val_ (h++lt1) p);
+  assert (theta (io_return val_) (h++lt1) p);
+  assert (thetaP (io_return val_) (h++lt1) lt2 fs_r);
+  assert (p lt2 fs_r);
+  assert (lt2 == []);
+  assert (fs_r == val_);
+  unit_l lt1;
+  eliminate forall (lt':local_trace h) (fs_r':get_Type t1). fs_beh fs_e' h lt' fs_r' ==> exists em'. t1 ∈ (h++lt', fs_r', em') /\ e_beh e em' h lt' with lt1 fs_v;
+  eliminate exists em'. t1 ∈ (h++lt1, fs_v, em') /\ e_beh e em' h lt1
+    returns exists e'. (t1 ^+ t2) ∈ (h++lt, fs_r, e') /\ e_beh (EInl e) e' h lt with _. begin
+  lem_values_are_values t1 (h++lt1) fs_v em';
+  lem_value_is_irred em';
+  lem_value_is_irred (EInl em');
+  FStar.Squash.bind_squash #(steps e em' h lt1) () (fun sts ->
+  construct_steps_einl e em' h lt1 sts)
+  end
+  end
+#pop-options
 
+#push-options "--z3rlimit 15"
+let helper_equiv_oprod_fmap_inr_steps (h:history) (lt:local_trace h) (t1 t2:qType)
+  (fs_e':fs_prod t2) (fs_r:fs_val (t1 ^+ t2)) (e:closed_exp) :
+  Lemma
+    (requires fs_beh (fs_prod_bind fs_e' (fun v -> return (Inr #(fs_val t1) #(fs_val t2) v))) h lt fs_r /\
+              t2 ⫃ (h, fs_e', e))
+    (ensures exists e'. (t1 ^+ t2) ∈ (h++lt, fs_r, e') /\ e_beh (EInr e) e' h lt) =
+  let fs_k : fs_val t2 -> fs_prod (t1 ^+ t2) = fun v -> return (Inr #(fs_val t1) #(fs_val t2) v) in
+  assert (fs_prod_bind fs_e' fs_k == io_bind fs_e' fs_k) by (norm [delta_only [`%fs_prod_bind]]; trefl ());
+  destruct_fs_beh fs_e' fs_k h lt fs_r;
+  eliminate exists (lt1:local_trace h) (lt2:local_trace (h++lt1)) (fs_v:fs_val t2).
+    lt == (lt1@lt2) /\ fs_beh fs_e' h lt1 fs_v /\ fs_beh (return (Inr #(fs_val t1) #(fs_val t2) fs_v)) (h++lt1) lt2 fs_r
+    returns exists e'. (t1 ^+ t2) ∈ (h++lt, fs_r, e') /\ e_beh (EInr e) e' h lt with _. begin
+  let val_ = Inr #(fs_val t1) #(fs_val t2) fs_v in
+  theta_monad_morphism_ret val_;
+  let p : hist_post (h++lt1) (get_Type (t1 ^+ t2)) = fun lt' r' -> lt' == [] /\ r' == val_ in
+  assert (hist_return val_ (h++lt1) p);
+  assert (theta (io_return val_) (h++lt1) p);
+  assert (thetaP (io_return val_) (h++lt1) lt2 fs_r);
+  assert (p lt2 fs_r);
+  assert (lt2 == []);
+  assert (fs_r == val_);
+  unit_l lt1;
+  eliminate forall (lt':local_trace h) (fs_r':get_Type t2). fs_beh fs_e' h lt' fs_r' ==> exists em'. t2 ∈ (h++lt', fs_r', em') /\ e_beh e em' h lt' with lt1 fs_v;
+  eliminate exists em'. t2 ∈ (h++lt1, fs_v, em') /\ e_beh e em' h lt1
+    returns exists e'. (t1 ^+ t2) ∈ (h++lt, fs_r, e') /\ e_beh (EInr e) e' h lt with _. begin
+  lem_values_are_values t2 (h++lt1) fs_v em';
+  lem_value_is_irred em';
+  lem_value_is_irred (EInr em');
+  FStar.Squash.bind_squash #(steps e em' h lt1) () (fun sts ->
+  construct_steps_einr e em' h lt1 sts)
+  end
+  end
+#pop-options
+
+#push-options "--z3rlimit 15"
+let helper_equiv_oprod_fmap_fst_steps (h:history) (lt:local_trace h) (t1 t2:qType)
+  (fs_e12':fs_prod (t1 ^* t2)) (fs_r:fs_val t1) (e12:closed_exp) :
+  Lemma
+    (requires fs_beh (fs_prod_bind fs_e12' (fun v -> return (fst #(fs_val t1) #(fs_val t2) v))) h lt fs_r /\
+              (t1 ^* t2) ⫃ (h, fs_e12', e12))
+    (ensures exists e'. t1 ∈ (h++lt, fs_r, e') /\ e_beh (EFst e12) e' h lt) =
+  let fs_k : fs_val (t1 ^* t2) -> fs_prod t1 = fun v -> return (fst #(fs_val t1) #(fs_val t2) v) in
+  assert (fs_prod_bind fs_e12' fs_k == io_bind fs_e12' fs_k) by (norm [delta_only [`%fs_prod_bind]]; trefl ());
+  destruct_fs_beh fs_e12' fs_k h lt fs_r;
+  eliminate exists (lt1:local_trace h) (lt2:local_trace (h++lt1)) (fs_pair:fs_val (t1 ^* t2)).
+    lt == (lt1@lt2) /\ fs_beh fs_e12' h lt1 fs_pair /\ fs_beh (return (fst #(fs_val t1) #(fs_val t2) fs_pair)) (h++lt1) lt2 fs_r
+    returns exists e'. t1 ∈ (h++lt, fs_r, e') /\ e_beh (EFst e12) e' h lt with _. begin
+  let val_ = fst #(fs_val t1) #(fs_val t2) fs_pair in
+  theta_monad_morphism_ret val_;
+  let p : hist_post (h++lt1) (get_Type t1) = fun lt' r' -> lt' == [] /\ r' == val_ in
+  assert (hist_return val_ (h++lt1) p);
+  assert (theta (io_return val_) (h++lt1) p);
+  assert (thetaP (io_return val_) (h++lt1) lt2 fs_r);
+  assert (p lt2 fs_r);
+  assert (lt2 == []);
+  assert (fs_r == val_);
+  unit_l lt1;
+  eliminate forall (lt':local_trace h) (fs_r':get_Type (t1 ^* t2)). fs_beh fs_e12' h lt' fs_r' ==> exists em'. (t1 ^* t2) ∈ (h++lt', fs_r', em') /\ e_beh e12 em' h lt' with lt1 fs_pair;
+  eliminate exists em'. (t1 ^* t2) ∈ (h++lt1, fs_pair, em') /\ e_beh e12 em' h lt1
+    returns exists e'. t1 ∈ (h++lt, fs_r, e') /\ e_beh (EFst e12) e' h lt with _. begin
+  lem_values_are_values (t1 ^* t2) (h++lt1) fs_pair em';
+  let EPair e1' e2' = em' in
+  lem_value_is_irred e1';
+  lem_value_is_irred e2';
+  // Construct: EFst e12 -->* EFst (EPair e1' e2') --> e1'
+  FStar.Squash.bind_squash #(steps e12 em' h lt1) () (fun sts ->
+  construct_steps_efst e12 em' h lt1 sts;
+  let _ : step (EFst (EPair e1' e2')) e1' (h++lt1) None = FstPairReturn (h++lt1) in
+  lem_step_implies_steps (EFst (EPair e1' e2')) e1' (h++lt1) None;
+  lem_steps_transitive (EFst e12) (EFst em') e1' h lt1 [];
+  unit_l lt1)
+  end
+  end
+#pop-options
+
+#push-options "--z3rlimit 15"
+let helper_equiv_oprod_fmap_snd_steps (h:history) (lt:local_trace h) (t1 t2:qType)
+  (fs_e12':fs_prod (t1 ^* t2)) (fs_r:fs_val t2) (e12:closed_exp) :
+  Lemma
+    (requires fs_beh (fs_prod_bind fs_e12' (fun v -> return (snd #(fs_val t1) #(fs_val t2) v))) h lt fs_r /\
+              (t1 ^* t2) ⫃ (h, fs_e12', e12))
+    (ensures exists e'. t2 ∈ (h++lt, fs_r, e') /\ e_beh (ESnd e12) e' h lt) =
+  let fs_k : fs_val (t1 ^* t2) -> fs_prod t2 = fun v -> return (snd #(fs_val t1) #(fs_val t2) v) in
+  assert (fs_prod_bind fs_e12' fs_k == io_bind fs_e12' fs_k) by (norm [delta_only [`%fs_prod_bind]]; trefl ());
+  destruct_fs_beh fs_e12' fs_k h lt fs_r;
+  eliminate exists (lt1:local_trace h) (lt2:local_trace (h++lt1)) (fs_pair:fs_val (t1 ^* t2)).
+    lt == (lt1@lt2) /\ fs_beh fs_e12' h lt1 fs_pair /\ fs_beh (return (snd #(fs_val t1) #(fs_val t2) fs_pair)) (h++lt1) lt2 fs_r
+    returns exists e'. t2 ∈ (h++lt, fs_r, e') /\ e_beh (ESnd e12) e' h lt with _. begin
+  let val_ = snd #(fs_val t1) #(fs_val t2) fs_pair in
+  theta_monad_morphism_ret val_;
+  let p : hist_post (h++lt1) (get_Type t2) = fun lt' r' -> lt' == [] /\ r' == val_ in
+  assert (hist_return val_ (h++lt1) p);
+  assert (theta (io_return val_) (h++lt1) p);
+  assert (thetaP (io_return val_) (h++lt1) lt2 fs_r);
+  assert (p lt2 fs_r);
+  assert (lt2 == []);
+  assert (fs_r == val_);
+  unit_l lt1;
+  eliminate forall (lt':local_trace h) (fs_r':get_Type (t1 ^* t2)). fs_beh fs_e12' h lt' fs_r' ==> exists em'. (t1 ^* t2) ∈ (h++lt', fs_r', em') /\ e_beh e12 em' h lt' with lt1 fs_pair;
+  eliminate exists em'. (t1 ^* t2) ∈ (h++lt1, fs_pair, em') /\ e_beh e12 em' h lt1
+    returns exists e'. t2 ∈ (h++lt, fs_r, e') /\ e_beh (ESnd e12) e' h lt with _. begin
+  lem_values_are_values (t1 ^* t2) (h++lt1) fs_pair em';
+  let EPair e1' e2' = em' in
+  lem_value_is_irred e1';
+  lem_value_is_irred e2';
+  FStar.Squash.bind_squash #(steps e12 em' h lt1) () (fun sts ->
+  construct_steps_esnd e12 em' h lt1 sts;
+  let _ : step (ESnd (EPair e1' e2')) e2' (h++lt1) None = SndPairReturn (h++lt1) in
+  lem_step_implies_steps (ESnd (EPair e1' e2')) e2' (h++lt1) None;
+  lem_steps_transitive (ESnd e12) (ESnd em') e2' h lt1 [];
+  unit_l lt1)
+  end
+  end
+#pop-options
+
+#push-options "--z3rlimit 15 --split_queries always"
+let helper_equiv_oprod_pair_steps (h:history) (lt:local_trace h) (t1 t2:qType)
+  (fs_e1':fs_prod t1) (fs_e2':fs_prod t2) (fs_r:fs_val (t1 ^* t2)) (e1 e2:closed_exp) :
+  Lemma
+    (requires fs_beh (fs_prod_bind fs_e1' (fun v1 -> fs_prod_bind #t2 #(t1 ^* t2) fs_e2' (fun v2 -> return (v1, v2)))) h lt fs_r /\
+              t1 ⫃ (h, fs_e1', e1) /\
+              (forall (lt':local_trace h). t2 ⫃ (h++lt', fs_e2', e2)))
+    (ensures exists e'. (t1 ^* t2) ∈ (h++lt, fs_r, e') /\ e_beh (EPair e1 e2) e' h lt) =
+  let fs_k1 : fs_val t1 -> fs_prod (t1 ^* t2) = fun v1 -> fs_prod_bind #t2 #(t1 ^* t2) fs_e2' (fun v2 -> return (v1, v2)) in
+  assert (fs_prod_bind fs_e1' fs_k1 == io_bind fs_e1' fs_k1) by (norm [delta_only [`%fs_prod_bind]]; trefl ());
+  destruct_fs_beh fs_e1' fs_k1 h lt fs_r;
+  eliminate exists (lt1:local_trace h) (lt2:local_trace (h++lt1)) (fs_v1:fs_val t1).
+    lt == (lt1@lt2) /\ fs_beh fs_e1' h lt1 fs_v1 /\ fs_beh (fs_k1 fs_v1) (h++lt1) lt2 fs_r
+    returns exists e'. (t1 ^* t2) ∈ (h++lt, fs_r, e') /\ e_beh (EPair e1 e2) e' h lt with _. begin
+  // Get e1 value
+  eliminate forall (lt':local_trace h) (fs_r':get_Type t1). fs_beh fs_e1' h lt' fs_r' ==> exists em'. t1 ∈ (h++lt', fs_r', em') /\ e_beh e1 em' h lt' with lt1 fs_v1;
+  eliminate exists em1. t1 ∈ (h++lt1, fs_v1, em1) /\ e_beh e1 em1 h lt1
+    returns exists e'. (t1 ^* t2) ∈ (h++lt, fs_r, e') /\ e_beh (EPair e1 e2) e' h lt with _. begin
+  lem_values_are_values t1 (h++lt1) fs_v1 em1;
+  lem_value_is_irred em1;
+  // Decompose inner bind: fs_prod_bind fs_e2' (fun v2 -> return (fs_v1, v2))
+  let fs_k2 : fs_val t2 -> fs_prod (t1 ^* t2) = fun v2 -> return (fs_v1, v2) in
+  assert (fs_prod_bind #t2 #(t1 ^* t2) fs_e2' fs_k2 == io_bind fs_e2' fs_k2) by (norm [delta_only [`%fs_prod_bind]]; trefl ());
+  destruct_fs_beh fs_e2' fs_k2 (h++lt1) lt2 fs_r;
+  eliminate exists (lt2a:local_trace (h++lt1)) (lt2b:local_trace ((h++lt1)++lt2a)) (fs_v2:fs_val t2).
+    lt2 == (lt2a@lt2b) /\ fs_beh fs_e2' (h++lt1) lt2a fs_v2 /\ fs_beh (return (fs_v1, fs_v2)) ((h++lt1)++lt2a) lt2b fs_r
+    returns exists e'. (t1 ^* t2) ∈ (h++lt, fs_r, e') /\ e_beh (EPair e1 e2) e' h lt with _. begin
+  let val_ = (fs_v1, fs_v2) in
+  theta_monad_morphism_ret val_;
+  let p : hist_post ((h++lt1)++lt2a) (get_Type (t1 ^* t2)) = fun lt' r' -> lt' == [] /\ r' == val_ in
+  assert (hist_return val_ ((h++lt1)++lt2a) p);
+  assert (theta (io_return val_) ((h++lt1)++lt2a) p);
+  assert (thetaP (io_return val_) ((h++lt1)++lt2a) lt2b fs_r);
+  assert (p lt2b fs_r);
+  assert (lt2b == []);
+  assert (fs_r == val_);
+  unit_l lt2a;
+  // Get e2 value
+  assert (t2 ⫃ (h++lt1, fs_e2', e2));
+  eliminate forall (lt':local_trace (h++lt1)) (fs_r':get_Type t2). fs_beh fs_e2' (h++lt1) lt' fs_r' ==> exists em'. t2 ∈ ((h++lt1)++lt', fs_r', em') /\ e_beh e2 em' (h++lt1) lt' with lt2a fs_v2;
+  eliminate exists em2. t2 ∈ ((h++lt1)++lt2a, fs_v2, em2) /\ e_beh e2 em2 (h++lt1) lt2a
+    returns exists e'. (t1 ^* t2) ∈ (h++lt, fs_r, e') /\ e_beh (EPair e1 e2) e' h lt with _. begin
+  lem_values_are_values t2 ((h++lt1)++lt2a) fs_v2 em2;
+  lem_value_is_irred em2;
+  trans_history h lt1 lt2a;
+  val_type_closed_under_history_extension t1 (h++lt1) fs_v1 em1;
+  lem_value_is_irred (EPair em1 em2);
+  // Construct: EPair e1 e2 -->* EPair em1 em2
+  FStar.Squash.bind_squash #(steps e1 em1 h lt1) () (fun sts1 ->
+  FStar.Squash.bind_squash #(steps e2 em2 (h++lt1) lt2a) () (fun sts2 ->
+  construct_steps_epair e1 em1 e2 em2 h lt1 lt2a sts1 sts2;
+  assert (steps (EPair e1 e2) (EPair em1 em2) h (lt1@lt2a))))
+  end
+  end
+  end
+  end
+#pop-options
+
+(** ---- Helpers for IO operation bind decomposition ---- **)
+
+#push-options "--z3rlimit 15"
+let helper_equiv_oprod_openfile_steps (h:history) (lt:local_trace h)
+  (fs_fnm':fs_prod qString) (fs_r:fs_val (qResexn qFileDescr)) (fnm:closed_exp) :
+  Lemma
+    (requires fs_beh (fs_prod_bind fs_fnm' (fun fnm' -> openfile fnm')) h lt fs_r /\
+              qString ⫃ (h, fs_fnm', fnm))
+    (ensures exists e'. (qResexn qFileDescr) ∈ (h++lt, fs_r, e') /\ e_beh (EOpen fnm) e' h lt) =
+  let fs_k : fs_val qString -> fs_prod (qResexn qFileDescr) = fun fnm' -> openfile fnm' in
+  assert (fs_prod_bind fs_fnm' fs_k == io_bind fs_fnm' fs_k) by (norm [delta_only [`%fs_prod_bind]]; trefl ());
+  destruct_fs_beh fs_fnm' fs_k h lt fs_r;
+  eliminate exists (lt1:local_trace h) (lt2:local_trace (h++lt1)) (fs_fnm_val:fs_val qString).
+    lt == (lt1@lt2) /\ fs_beh fs_fnm' h lt1 fs_fnm_val /\ fs_beh (openfile fs_fnm_val) (h++lt1) lt2 fs_r
+    returns exists e'. (qResexn qFileDescr) ∈ (h++lt, fs_r, e') /\ e_beh (EOpen fnm) e' h lt with _. begin
+  eliminate forall (lt':local_trace h) (fs_r':get_Type qString). fs_beh fs_fnm' h lt' fs_r' ==> exists em'. qString ∈ (h++lt', fs_r', em') /\ e_beh fnm em' h lt' with lt1 fs_fnm_val;
+  eliminate exists em'. qString ∈ (h++lt1, fs_fnm_val, em') /\ e_beh fnm em' h lt1
+    returns exists e'. (qResexn qFileDescr) ∈ (h++lt, fs_r, e') /\ e_beh (EOpen fnm) e' h lt with _. begin
+  lem_values_are_values qString (h++lt1) fs_fnm_val em';
+  trans_history h lt1 lt2;
+  helper_equiv_oprod_openfile_oval_steps (h++lt1) lt2 fs_fnm_val em' fs_r;
+  eliminate exists e'. (qResexn qFileDescr) ∈ ((h++lt1)++lt2, fs_r, e') /\ e_beh (EOpen em') e' (h++lt1) lt2
+    returns exists e'. (qResexn qFileDescr) ∈ (h++lt, fs_r, e') /\ e_beh (EOpen fnm) e' h lt with _. begin
+  FStar.Squash.bind_squash #(steps fnm em' h lt1) () (fun sts_fnm ->
+  FStar.Squash.bind_squash #(steps (EOpen em') e' (h++lt1) lt2) () (fun sts_open ->
+  construct_steps_eopen fnm em' h lt1 sts_fnm;
+  lem_steps_transitive (EOpen fnm) (EOpen em') e' h lt1 lt2))
+  end
+  end
+  end
+#pop-options
+
+#push-options "--z3rlimit 15"
+let helper_equiv_oprod_read_steps (h:history) (lt:local_trace h)
+  (fs_fd':fs_prod qFileDescr) (fs_r:fs_val (qResexn qString)) (fd:closed_exp) :
+  Lemma
+    (requires fs_beh (fs_prod_bind fs_fd' (fun fd' -> read fd')) h lt fs_r /\
+              qFileDescr ⫃ (h, fs_fd', fd))
+    (ensures exists e'. (qResexn qString) ∈ (h++lt, fs_r, e') /\ e_beh (ERead fd) e' h lt) =
+  let fs_k : fs_val qFileDescr -> fs_prod (qResexn qString) = fun fd' -> read fd' in
+  assert (fs_prod_bind fs_fd' fs_k == io_bind fs_fd' fs_k) by (norm [delta_only [`%fs_prod_bind]]; trefl ());
+  destruct_fs_beh fs_fd' fs_k h lt fs_r;
+  eliminate exists (lt1:local_trace h) (lt2:local_trace (h++lt1)) (fs_fd_val:fs_val qFileDescr).
+    lt == (lt1@lt2) /\ fs_beh fs_fd' h lt1 fs_fd_val /\ fs_beh (read fs_fd_val) (h++lt1) lt2 fs_r
+    returns exists e'. (qResexn qString) ∈ (h++lt, fs_r, e') /\ e_beh (ERead fd) e' h lt with _. begin
+  eliminate forall (lt':local_trace h) (fs_r':get_Type qFileDescr). fs_beh fs_fd' h lt' fs_r' ==> exists em'. qFileDescr ∈ (h++lt', fs_r', em') /\ e_beh fd em' h lt' with lt1 fs_fd_val;
+  eliminate exists em'. qFileDescr ∈ (h++lt1, fs_fd_val, em') /\ e_beh fd em' h lt1
+    returns exists e'. (qResexn qString) ∈ (h++lt, fs_r, e') /\ e_beh (ERead fd) e' h lt with _. begin
+  lem_values_are_values qFileDescr (h++lt1) fs_fd_val em';
+  trans_history h lt1 lt2;
+  helper_equiv_oprod_read_oval_steps (h++lt1) lt2 fs_fd_val em' fs_r;
+  eliminate exists e'. (qResexn qString) ∈ ((h++lt1)++lt2, fs_r, e') /\ e_beh (ERead em') e' (h++lt1) lt2
+    returns exists e'. (qResexn qString) ∈ (h++lt, fs_r, e') /\ e_beh (ERead fd) e' h lt with _. begin
+  FStar.Squash.bind_squash #(steps fd em' h lt1) () (fun sts_fd ->
+  FStar.Squash.bind_squash #(steps (ERead em') e' (h++lt1) lt2) () (fun sts_read ->
+  construct_steps_eread fd em' h lt1 sts_fd;
+  lem_steps_transitive (ERead fd) (ERead em') e' h lt1 lt2))
+  end
+  end
+  end
+#pop-options
+
+#push-options "--z3rlimit 15"
+let helper_equiv_oprod_close_steps (h:history) (lt:local_trace h)
+  (fs_fd':fs_prod qFileDescr) (fs_r:fs_val (qResexn qUnit)) (fd:closed_exp) :
+  Lemma
+    (requires fs_beh (fs_prod_bind fs_fd' (fun fd' -> close fd')) h lt fs_r /\
+              qFileDescr ⫃ (h, fs_fd', fd))
+    (ensures exists e'. (qResexn qUnit) ∈ (h++lt, fs_r, e') /\ e_beh (EClose fd) e' h lt) =
+  let fs_k : fs_val qFileDescr -> fs_prod (qResexn qUnit) = fun fd' -> close fd' in
+  assert (fs_prod_bind fs_fd' fs_k == io_bind fs_fd' fs_k) by (norm [delta_only [`%fs_prod_bind]]; trefl ());
+  destruct_fs_beh fs_fd' fs_k h lt fs_r;
+  eliminate exists (lt1:local_trace h) (lt2:local_trace (h++lt1)) (fs_fd_val:fs_val qFileDescr).
+    lt == (lt1@lt2) /\ fs_beh fs_fd' h lt1 fs_fd_val /\ fs_beh (close fs_fd_val) (h++lt1) lt2 fs_r
+    returns exists e'. (qResexn qUnit) ∈ (h++lt, fs_r, e') /\ e_beh (EClose fd) e' h lt with _. begin
+  eliminate forall (lt':local_trace h) (fs_r':get_Type qFileDescr). fs_beh fs_fd' h lt' fs_r' ==> exists em'. qFileDescr ∈ (h++lt', fs_r', em') /\ e_beh fd em' h lt' with lt1 fs_fd_val;
+  eliminate exists em'. qFileDescr ∈ (h++lt1, fs_fd_val, em') /\ e_beh fd em' h lt1
+    returns exists e'. (qResexn qUnit) ∈ (h++lt, fs_r, e') /\ e_beh (EClose fd) e' h lt with _. begin
+  lem_values_are_values qFileDescr (h++lt1) fs_fd_val em';
+  trans_history h lt1 lt2;
+  helper_equiv_oprod_close_oval_steps (h++lt1) lt2 fs_fd_val em' fs_r;
+  eliminate exists e'. (qResexn qUnit) ∈ ((h++lt1)++lt2, fs_r, e') /\ e_beh (EClose em') e' (h++lt1) lt2
+    returns exists e'. (qResexn qUnit) ∈ (h++lt, fs_r, e') /\ e_beh (EClose fd) e' h lt with _. begin
+  FStar.Squash.bind_squash #(steps fd em' h lt1) () (fun sts_fd ->
+  FStar.Squash.bind_squash #(steps (EClose em') e' (h++lt1) lt2) () (fun sts_close ->
+  construct_steps_eclose fd em' h lt1 sts_fd;
+  lem_steps_transitive (EClose fd) (EClose em') e' h lt1 lt2))
+  end
+  end
+  end
+#pop-options
+
+#push-options "--z3rlimit 15 --split_queries always"
+let helper_equiv_oprod_write_steps (h:history) (lt:local_trace h)
+  (fs_fd':fs_prod qFileDescr) (fs_msg':fs_prod qString) (fs_r:fs_val (qResexn qUnit)) (fd msg:closed_exp) :
+  Lemma
+    (requires fs_beh (fs_prod_bind fs_fd' (fun fd' -> fs_prod_bind #qString #(qResexn qUnit) fs_msg' (fun msg' -> write (fd', msg')))) h lt fs_r /\
+              qFileDescr ⫃ (h, fs_fd', fd) /\
+              (forall (lt':local_trace h). qString ⫃ (h++lt', fs_msg', msg)))
+    (ensures exists e'. (qResexn qUnit) ∈ (h++lt, fs_r, e') /\ e_beh (EWrite fd msg) e' h lt) =
+  let fs_k1 : fs_val qFileDescr -> fs_prod (qResexn qUnit) = fun fd' -> fs_prod_bind #qString #(qResexn qUnit) fs_msg' (fun msg' -> write (fd', msg')) in
+  assert (fs_prod_bind fs_fd' fs_k1 == io_bind fs_fd' fs_k1) by (norm [delta_only [`%fs_prod_bind]]; trefl ());
+  destruct_fs_beh fs_fd' fs_k1 h lt fs_r;
+  eliminate exists (lt1:local_trace h) (lt2:local_trace (h++lt1)) (fs_fd_val:fs_val qFileDescr).
+    lt == (lt1@lt2) /\ fs_beh fs_fd' h lt1 fs_fd_val /\ fs_beh (fs_k1 fs_fd_val) (h++lt1) lt2 fs_r
+    returns exists e'. (qResexn qUnit) ∈ (h++lt, fs_r, e') /\ e_beh (EWrite fd msg) e' h lt with _. begin
+  // Get fd value
+  eliminate forall (lt':local_trace h) (fs_r':get_Type qFileDescr). fs_beh fs_fd' h lt' fs_r' ==> exists em'. qFileDescr ∈ (h++lt', fs_r', em') /\ e_beh fd em' h lt' with lt1 fs_fd_val;
+  eliminate exists em_fd. qFileDescr ∈ (h++lt1, fs_fd_val, em_fd) /\ e_beh fd em_fd h lt1
+    returns exists e'. (qResexn qUnit) ∈ (h++lt, fs_r, e') /\ e_beh (EWrite fd msg) e' h lt with _. begin
+  lem_values_are_values qFileDescr (h++lt1) fs_fd_val em_fd;
+  lem_value_is_irred em_fd;
+  // Decompose inner bind: fs_prod_bind fs_msg' (fun msg' -> write (fs_fd_val, msg'))
+  let fs_k2 : fs_val qString -> fs_prod (qResexn qUnit) = fun msg' -> write (fs_fd_val, msg') in
+  assert (fs_prod_bind #qString #(qResexn qUnit) fs_msg' fs_k2 == io_bind fs_msg' fs_k2) by (norm [delta_only [`%fs_prod_bind]]; trefl ());
+  destruct_fs_beh fs_msg' fs_k2 (h++lt1) lt2 fs_r;
+  eliminate exists (lt2a:local_trace (h++lt1)) (lt2b:local_trace ((h++lt1)++lt2a)) (fs_msg_val:fs_val qString).
+    lt2 == (lt2a@lt2b) /\ fs_beh fs_msg' (h++lt1) lt2a fs_msg_val /\ fs_beh (write (fs_fd_val, fs_msg_val)) ((h++lt1)++lt2a) lt2b fs_r
+    returns exists e'. (qResexn qUnit) ∈ (h++lt, fs_r, e') /\ e_beh (EWrite fd msg) e' h lt with _. begin
+  // Get msg value
+  assert (qString ⫃ (h++lt1, fs_msg', msg));
+  eliminate forall (lt':local_trace (h++lt1)) (fs_r':get_Type qString). fs_beh fs_msg' (h++lt1) lt' fs_r' ==> exists em'. qString ∈ ((h++lt1)++lt', fs_r', em') /\ e_beh msg em' (h++lt1) lt' with lt2a fs_msg_val;
+  eliminate exists em_msg. qString ∈ ((h++lt1)++lt2a, fs_msg_val, em_msg) /\ e_beh msg em_msg (h++lt1) lt2a
+    returns exists e'. (qResexn qUnit) ∈ (h++lt, fs_r, e') /\ e_beh (EWrite fd msg) e' h lt with _. begin
+  lem_values_are_values qString ((h++lt1)++lt2a) fs_msg_val em_msg;
+  trans_history h lt1 lt2a;
+  trans_history (h++lt1) lt2a lt2b;
+  trans_history h lt1 lt2;
+  associative_history lt1 lt2a lt2b;
+  // Use existing write oval helper at history (h++lt1)++lt2a
+  val_type_closed_under_history_extension qFileDescr (h++lt1) fs_fd_val em_fd;
+  helper_equiv_oprod_write_oval_steps ((h++lt1)++lt2a) lt2b fs_fd_val fs_msg_val em_fd em_msg fs_r;
+  eliminate exists e'. (qResexn qUnit) ∈ (((h++lt1)++lt2a)++lt2b, fs_r, e') /\ e_beh (EWrite em_fd em_msg) e' ((h++lt1)++lt2a) lt2b
+    returns exists e'. (qResexn qUnit) ∈ (h++lt, fs_r, e') /\ e_beh (EWrite fd msg) e' h lt with _. begin
+  // Construct: EWrite fd msg -->* EWrite em_fd msg -->* EWrite em_fd em_msg -->* e'
+  FStar.Squash.bind_squash #(steps fd em_fd h lt1) () (fun sts_fd ->
+  construct_steps_ewrite_fd fd em_fd msg h lt1 sts_fd;
+  FStar.Squash.bind_squash #(steps msg em_msg (h++lt1) lt2a) () (fun sts_msg ->
+  construct_steps_ewrite_arg em_fd msg em_msg (h++lt1) lt2a sts_msg;
+  lem_steps_transitive (EWrite fd msg) (EWrite em_fd msg) (EWrite em_fd em_msg) h lt1 lt2a;
+  FStar.Squash.bind_squash #(steps (EWrite em_fd em_msg) e' ((h++lt1)++lt2a) lt2b) () (fun sts_wr ->
+  lem_steps_transitive (EWrite fd msg) (EWrite em_fd em_msg) e' h (lt1@lt2a) lt2b)))
+  end
+  end
+  end
+  end
+  end
+#pop-options
+
+(** ---- Case helper for bind decomposition ---- **)
+
+#push-options "--z3rlimit 15"
+let helper_equiv_oprod_case_steps (h:history) (lt:local_trace h) (a b c:qType)
+  (fs_sc':fs_prod (a ^+ b))
+  (fs_inlc:fs_val (a ^->!@ c))
+  (fs_inrc:fs_val (b ^->!@ c))
+  (fs_r:fs_val c)
+  (e_sc:closed_exp)
+  (e_lc:exp{is_closed (ELam e_lc)})
+  (e_rc:exp{is_closed (ELam e_rc)}) :
+  Lemma
+    (requires fs_beh (fs_prod_bind fs_sc' (fun x -> fs_prod_case_val x fs_inlc fs_inrc)) h lt fs_r /\
+              (a ^+ b) ⫃ (h, fs_sc', e_sc) /\
+              (a ^->!@ c) ⊆ (h, fs_inlc, ELam e_lc) /\
+              (b ^->!@ c) ⊆ (h, fs_inrc, ELam e_rc))
+    (ensures exists e'. c ∈ (h++lt, fs_r, e') /\ e_beh (ECase e_sc e_lc e_rc) e' h lt) =
+  let fs_k : fs_val (a ^+ b) -> fs_prod c = fun x -> fs_prod_case_val x fs_inlc fs_inrc in
+  assert (fs_prod_bind fs_sc' fs_k == io_bind fs_sc' fs_k) by (norm [delta_only [`%fs_prod_bind]]; trefl ());
+  destruct_fs_beh fs_sc' fs_k h lt fs_r;
+  eliminate exists (lt1:local_trace h) (lt2:local_trace (h++lt1)) (fs_cond_val:fs_val (a ^+ b)).
+    lt == (lt1@lt2) /\ fs_beh fs_sc' h lt1 fs_cond_val /\ fs_beh (fs_prod_case_val fs_cond_val fs_inlc fs_inrc) (h++lt1) lt2 fs_r
+    returns exists e'. c ∈ (h++lt, fs_r, e') /\ e_beh (ECase e_sc e_lc e_rc) e' h lt with _. begin
+  // Get condition value
+  eliminate forall (lt':local_trace h) (fs_r':get_Type (a ^+ b)). fs_beh fs_sc' h lt' fs_r' ==> exists em'. (a ^+ b) ∈ (h++lt', fs_r', em') /\ e_beh e_sc em' h lt' with lt1 fs_cond_val;
+  eliminate exists em'. (a ^+ b) ∈ (h++lt1, fs_cond_val, em') /\ e_beh e_sc em' h lt1
+    returns exists e'. c ∈ (h++lt, fs_r, e') /\ e_beh (ECase e_sc e_lc e_rc) e' h lt with _. begin
+  lem_values_are_values (a ^+ b) (h++lt1) fs_cond_val em';
+  trans_history h lt1 lt2;
+  // Convert (a ^+ b) ∈ to ⊆ at h++lt1
+  lem_values_are_expressions (a ^+ b) (h++lt1) fs_cond_val em';
+  // Shift ⊆ for inlc from h to h++lt1
+  eliminate exists (elc':closed_exp). e_beh (ELam e_lc) elc' h [] /\ (a ^->!@ c) ∈ (h, fs_inlc, elc')
+    returns (a ^->!@ c) ⊆ (h++lt1, fs_inlc, ELam e_lc) with _. begin
+  steps_val_id (ELam e_lc) elc' h;
+  val_type_closed_under_history_extension (a ^->!@ c) h fs_inlc (ELam e_lc);
+  lem_values_are_expressions (a ^->!@ c) (h++lt1) fs_inlc (ELam e_lc)
+  end;
+  // Shift ⊆ for inrc from h to h++lt1
+  eliminate exists (erc':closed_exp). e_beh (ELam e_rc) erc' h [] /\ (b ^->!@ c) ∈ (h, fs_inrc, erc')
+    returns (b ^->!@ c) ⊆ (h++lt1, fs_inrc, ELam e_rc) with _. begin
+  steps_val_id (ELam e_rc) erc' h;
+  val_type_closed_under_history_extension (b ^->!@ c) h fs_inrc (ELam e_rc);
+  lem_values_are_expressions (b ^->!@ c) (h++lt1) fs_inrc (ELam e_rc)
+  end;
+  helper_equiv_oprod_case_oval_steps (h++lt1) lt2 a b c fs_cond_val fs_inlc fs_inrc fs_r em' e_lc e_rc;
+  eliminate exists e'. c ∈ ((h++lt1)++lt2, fs_r, e') /\ e_beh (ECase em' e_lc e_rc) e' (h++lt1) lt2
+    returns exists e'. c ∈ (h++lt, fs_r, e') /\ e_beh (ECase e_sc e_lc e_rc) e' h lt with _. begin
+  FStar.Squash.bind_squash #(steps e_sc em' h lt1) () (fun sts_cond ->
+  FStar.Squash.bind_squash #(steps (ECase em' e_lc e_rc) e' (h++lt1) lt2) () (fun sts_case ->
+  construct_steps_ecase_cond e_sc em' e_lc e_rc h lt1 sts_cond;
+  lem_steps_transitive (ECase e_sc e_lc e_rc) (ECase em' e_lc e_rc) e' h lt1 lt2))
+  end
+  end
+  end
+#pop-options
+
+(** ---- Main compatibility lemma proofs ---- **)
+
+#push-options "--split_queries always"
 let equiv_oprod_pair #g
   (#t1 #t2:qType)
   (fs_e1:fs_oprod g t1) (fs_e2:fs_oprod g t2)
@@ -1111,8 +1642,32 @@ let equiv_oprod_pair #g
   : Lemma
     (requires fs_e1 ⊑ e1 /\ fs_e2 ⊑ e2)
     (ensures fs_oprod_pair fs_e1 fs_e2 ⊑ EPair e1 e2) =
-  admit ()
+  lem_fv_in_env_pair g e1 e2;
+  introduce forall b' (s:gsub g b') fsG h. fsG `(≍) h` s ==> (t1 ^* t2) ⫃ (h, fs_oprod_pair fs_e1 fs_e2 fsG, gsubst s (EPair e1 e2)) with begin
+    introduce _ ==> _ with _. begin
+      let fs_e1' : fs_prod t1 = fs_e1 fsG in
+      let fs_e2' : fs_prod t2 = fs_e2 fsG in
+      let fs_e = fs_prod_bind fs_e1' (fun v1 -> fs_prod_bind #t2 #(t1 ^* t2) fs_e2' (fun v2 -> return (v1, v2))) in
+      assert (fs_e == fs_oprod_pair fs_e1 fs_e2 fsG) by (
+        norm [delta_only [`%fs_oprod_pair;`%fs_oprod_bind';`%fs_oprod_bind;`%fs_oprod_return_val;`%fs_val_pair]];
+        l_to_r [`lem_hd_stack;`tail_stack_inverse];
+        trefl ());
+      let e = EPair (gsubst s e1) (gsubst s e2) in
+      assert (gsubst s (EPair e1 e2) == e);
+      let EPair e1 e2 = e in
+      introduce fsG `(≍) h` s ==> (t1 ^* t2) ⫃ (h, fs_e, e) with _. begin
+        lem_shift_type_value_environments h fsG s;
+        introduce forall lt (fs_r:fs_val (t1 ^* t2)). fs_beh fs_e h lt fs_r ==> exists e'. (t1 ^* t2) ∈ (h++lt, fs_r, e') /\ e_beh e e' h lt with begin
+          introduce fs_beh fs_e h lt fs_r ==> exists e'. (t1 ^* t2) ∈ (h++lt, fs_r, e') /\ e_beh e e' h lt with _. begin
+            helper_equiv_oprod_pair_steps h lt t1 t2 fs_e1' fs_e2' fs_r e1 e2
+          end
+        end
+      end
+    end
+  end
+#pop-options
 
+#push-options "--split_queries always"
 let equiv_oprod_fst #g
   (#t1 #t2:qType)
   (fs_e12:fs_oprod g (t1 ^* t2))
@@ -1120,14 +1675,61 @@ let equiv_oprod_fst #g
   : Lemma
     (requires fs_e12 ⊑ e12) (** is this too strict? we only care for the left to be equivalent. **)
     (ensures fs_oprod_fmap fs_e12 fst ⊑ (EFst e12))
-  = admit ()
+  =
+  lem_fv_in_env_fst g e12;
+  introduce forall b' (s:gsub g b') fsG h. fsG `(≍) h` s ==> t1 ⫃ (h, (fs_oprod_fmap #g #(t1 ^* t2) #t1 fs_e12 fst) fsG, gsubst s (EFst e12)) with begin
+    introduce _ ==> _ with _. begin
+      let fs_e12' : fs_prod (t1 ^* t2) = fs_e12 fsG in
+      let fs_e = fs_prod_bind #(t1 ^* t2) #t1 fs_e12' (fun v -> return (fst #(fs_val t1) #(fs_val t2) v)) in
+      assert (fs_e == (fs_oprod_fmap #g #(t1 ^* t2) #t1 fs_e12 fst) fsG) by (
+        norm [delta_only [`%fs_oprod_fmap;`%fs_oprod_bind';`%fs_oprod_bind;`%fs_oprod_return_val]];
+        l_to_r [`lem_hd_stack;`tail_stack_inverse];
+        trefl ());
+      let e = EFst (gsubst s e12) in
+      assert (gsubst s (EFst e12) == e);
+      let EFst e12 = e in
+      introduce fsG `(≍) h` s ==> t1 ⫃ (h, fs_e, e) with _. begin
+        lem_shift_type_value_environments h fsG s;
+        introduce forall lt (fs_r:fs_val t1). fs_beh fs_e h lt fs_r ==> exists e'. t1 ∈ (h++lt, fs_r, e') /\ e_beh e e' h lt with begin
+          introduce fs_beh fs_e h lt fs_r ==> exists e'. t1 ∈ (h++lt, fs_r, e') /\ e_beh e e' h lt with _. begin
+            helper_equiv_oprod_fmap_fst_steps h lt t1 t2 fs_e12' fs_r e12
+          end
+        end
+      end
+    end
+  end
+#pop-options
 
+#push-options "--split_queries always"
 let equiv_oprod_snd #g (#t1 #t2:qType) (fs_e12:fs_oprod g (t1 ^* t2)) (e12:exp)
   : Lemma
     (requires fs_e12 ⊑ e12) (** is this too strict? we only care for the left to be equivalent. **)
     (ensures fs_oprod_fmap fs_e12 snd ⊑ (ESnd e12)) =
-  admit ()
+  lem_fv_in_env_snd g e12;
+  introduce forall b' (s:gsub g b') fsG h. fsG `(≍) h` s ==> t2 ⫃ (h, (fs_oprod_fmap #g #(t1 ^* t2) #t2 fs_e12 snd) fsG, gsubst s (ESnd e12)) with begin
+    introduce _ ==> _ with _. begin
+      let fs_e12' : fs_prod (t1 ^* t2) = fs_e12 fsG in
+      let fs_e = fs_prod_bind #(t1 ^* t2) #t2 fs_e12' (fun v -> return (snd #(fs_val t1) #(fs_val t2) v)) in
+      assert (fs_e == (fs_oprod_fmap #g #(t1 ^* t2) #t2 fs_e12 snd) fsG) by (
+        norm [delta_only [`%fs_oprod_fmap;`%fs_oprod_bind';`%fs_oprod_bind;`%fs_oprod_return_val]];
+        l_to_r [`lem_hd_stack;`tail_stack_inverse];
+        trefl ());
+      let e = ESnd (gsubst s e12) in
+      assert (gsubst s (ESnd e12) == e);
+      let ESnd e12 = e in
+      introduce fsG `(≍) h` s ==> t2 ⫃ (h, fs_e, e) with _. begin
+        lem_shift_type_value_environments h fsG s;
+        introduce forall lt (fs_r:fs_val t2). fs_beh fs_e h lt fs_r ==> exists e'. t2 ∈ (h++lt, fs_r, e') /\ e_beh e e' h lt with begin
+          introduce fs_beh fs_e h lt fs_r ==> exists e'. t2 ∈ (h++lt, fs_r, e') /\ e_beh e e' h lt with _. begin
+            helper_equiv_oprod_fmap_snd_steps h lt t1 t2 fs_e12' fs_r e12
+          end
+        end
+      end
+    end
+  end
+#pop-options
 
+#push-options "--split_queries always"
 let equiv_oprod_case #g (#a #b #c:qType)
   (fs_cond:fs_oprod g (a ^+ b))
   (fs_inlc:fs_oprod (extend a g) c)
@@ -1136,28 +1738,213 @@ let equiv_oprod_case #g (#a #b #c:qType)
   : Lemma
     (requires fs_cond ⊑ cond /\ fs_inlc ⊑ inlc /\ fs_inrc ⊑ inrc)
     (ensures (fs_oprod_case fs_cond fs_inlc fs_inrc) ⊑ (ECase cond inlc inrc)) =
-  admit ()
+  lem_fv_in_env_case g a b cond inlc inrc;
+  lem_fv_in_env_lam g a inlc;
+  lem_fv_in_env_lam g b inrc;
+  equiv_oval_lambda_oprod fs_inlc inlc;
+  equiv_oval_lambda_oprod fs_inrc inrc;
+  introduce forall b' (s:gsub g b') fsG h. fsG `(≍) h` s ==> c ⫃ (h, fs_oprod_case fs_cond fs_inlc fs_inrc fsG, gsubst s (ECase cond inlc inrc)) with begin
+    introduce _ ==> _ with _. begin
+      let fs_sc : fs_prod (a ^+ b) = fs_cond fsG in
+      let fs_il : fs_val (a ^->!@ c) = fun x -> fs_inlc (stack fsG x) in
+      let fs_ir : fs_val (b ^->!@ c) = fun x -> fs_inrc (stack fsG x) in
+      let fs_e = fs_prod_bind fs_sc (fun x -> fs_prod_case_val x fs_il fs_ir) in
+      assert (fs_e == fs_oprod_case fs_cond fs_inlc fs_inrc fsG) by (
+        norm [delta_only [`%fs_oprod_case;`%fs_prod_case_val;`%fs_oprod_bind';`%fs_oprod_bind;`%fs_oprod_case_val]];
+        l_to_r [`lem_hd_stack;`tail_stack_inverse];
+        trefl ());
+      let e = ECase (gsubst s cond) (subst (sub_elam s) inlc) (subst (sub_elam s) inrc) in
+      assert (gsubst s (ECase cond inlc inrc) == e);
+      let ECase e_sc e_il e_ir = e in
+      introduce fsG `(≍) h` s ==> c ⫃ (h, fs_e, e) with _. begin
+        lem_shift_type_value_environments h fsG s;
+        introduce forall lt (fs_r:fs_val c). fs_beh fs_e h lt fs_r ==> exists e'. c ∈ (h++lt, fs_r, e') /\ e_beh e e' h lt with begin
+          introduce fs_beh fs_e h lt fs_r ==> exists e'. c ∈ (h++lt, fs_r, e') /\ e_beh e e' h lt with _. begin
+            helper_equiv_oprod_case_steps h lt a b c fs_sc fs_il fs_ir fs_r e_sc e_il e_ir
+          end
+        end
+      end
+    end
+  end
+#pop-options
 
+#push-options "--split_queries always"
+let equiv_oprod_inl #g (t1 t2:qType) (fs_e:fs_oprod g t1) (e:exp)
+  : Lemma
+    (requires fs_e ⊑ e)
+    (ensures fs_oprod_fmap #g #t1 #(t1 ^+ t2) fs_e Inl ⊑ (EInl e))
+  =
+  lem_fv_in_env_inl g e;
+  introduce forall b' (s:gsub g b') fsG h. fsG `(≍) h` s ==> (t1 ^+ t2) ⫃ (h, (fs_oprod_fmap #g #t1 #(t1 ^+ t2) fs_e Inl) fsG, gsubst s (EInl e)) with begin
+    introduce _ ==> _ with _. begin
+      let fs_e' : fs_prod t1 = fs_e fsG in
+      let fs_ex = fs_prod_bind #t1 #(t1 ^+ t2) fs_e' (fun v -> return (Inl #(fs_val t1) #(fs_val t2) v)) in
+      assert (fs_ex == (fs_oprod_fmap #g #t1 #(t1 ^+ t2) fs_e Inl) fsG) by (
+        norm [delta_only [`%fs_oprod_fmap;`%fs_oprod_bind';`%fs_oprod_bind;`%fs_oprod_return_val]];
+        l_to_r [`lem_hd_stack;`tail_stack_inverse];
+        trefl ());
+      let ex = EInl (gsubst s e) in
+      assert (gsubst s (EInl e) == ex);
+      let EInl e = ex in
+      introduce fsG `(≍) h` s ==> (t1 ^+ t2) ⫃ (h, fs_ex, ex) with _. begin
+        lem_shift_type_value_environments h fsG s;
+        introduce forall lt (fs_r:fs_val (t1 ^+ t2)). fs_beh fs_ex h lt fs_r ==> exists e'. (t1 ^+ t2) ∈ (h++lt, fs_r, e') /\ e_beh ex e' h lt with begin
+          introduce fs_beh fs_ex h lt fs_r ==> exists e'. (t1 ^+ t2) ∈ (h++lt, fs_r, e') /\ e_beh ex e' h lt with _. begin
+            helper_equiv_oprod_fmap_inl_steps h lt t1 t2 fs_e' fs_r e
+          end
+        end
+      end
+    end
+  end
+#pop-options
+
+#push-options "--split_queries always"
+let equiv_oprod_inr #g (t1 t2:qType) (fs_e:fs_oprod g t2) (e:exp)
+  : Lemma
+    (requires fs_e ⊑ e)
+    (ensures fs_oprod_fmap #g #t2 #(t1 ^+ t2) fs_e Inr ⊑ (EInr e))
+  =
+  lem_fv_in_env_inr g e;
+  introduce forall b' (s:gsub g b') fsG h. fsG `(≍) h` s ==> (t1 ^+ t2) ⫃ (h, (fs_oprod_fmap #g #t2 #(t1 ^+ t2) fs_e Inr) fsG, gsubst s (EInr e)) with begin
+    introduce _ ==> _ with _. begin
+      let fs_e' : fs_prod t2 = fs_e fsG in
+      let fs_ex = fs_prod_bind #t2 #(t1 ^+ t2) fs_e' (fun v -> return (Inr #(fs_val t1) #(fs_val t2) v)) in
+      assert (fs_ex == (fs_oprod_fmap #g #t2 #(t1 ^+ t2) fs_e Inr) fsG) by (
+        norm [delta_only [`%fs_oprod_fmap;`%fs_oprod_bind';`%fs_oprod_bind;`%fs_oprod_return_val]];
+        l_to_r [`lem_hd_stack;`tail_stack_inverse];
+        trefl ());
+      let ex = EInr (gsubst s e) in
+      assert (gsubst s (EInr e) == ex);
+      let EInr e = ex in
+      introduce fsG `(≍) h` s ==> (t1 ^+ t2) ⫃ (h, fs_ex, ex) with _. begin
+        lem_shift_type_value_environments h fsG s;
+        introduce forall lt (fs_r:fs_val (t1 ^+ t2)). fs_beh fs_ex h lt fs_r ==> exists e'. (t1 ^+ t2) ∈ (h++lt, fs_r, e') /\ e_beh ex e' h lt with begin
+          introduce fs_beh fs_ex h lt fs_r ==> exists e'. (t1 ^+ t2) ∈ (h++lt, fs_r, e') /\ e_beh ex e' h lt with _. begin
+            helper_equiv_oprod_fmap_inr_steps h lt t1 t2 fs_e' fs_r e
+          end
+        end
+      end
+    end
+  end
+#pop-options
+
+#push-options "--split_queries always"
 let equiv_oprod_openfile #g (fs_fnm:fs_oprod g qString) (fnm:exp)
   : Lemma
     (requires fs_fnm ⊑ fnm)
     (ensures fs_oprod_openfile fs_fnm ⊑ EOpen fnm)
-  = admit ()
+  =
+  lem_fv_in_env_openfile g fnm;
+  introduce forall b' (s:gsub g b') fsG h. fsG `(≍) h` s ==> (qResexn qFileDescr) ⫃ (h, (fs_oprod_openfile fs_fnm) fsG, gsubst s (EOpen fnm)) with begin
+    introduce _ ==> _ with _. begin
+      let fs_fnm' : fs_prod qString = fs_fnm fsG in
+      let fs_e = fs_prod_bind fs_fnm' (fun fnm' -> openfile fnm') in
+      assert (fs_e == (fs_oprod_openfile fs_fnm) fsG) by (
+        norm [delta_only [`%fs_oprod_openfile;`%fs_oprod_bind';`%fs_oprod_bind;`%fs_oprod_return_prod]];
+        l_to_r [`lem_hd_stack;`tail_stack_inverse];
+        trefl ());
+      let e = EOpen (gsubst s fnm) in
+      assert (gsubst s (EOpen fnm) == e);
+      let EOpen fnm = e in
+      introduce fsG `(≍) h` s ==> (qResexn qFileDescr) ⫃ (h, fs_e, e) with _. begin
+        lem_shift_type_value_environments h fsG s;
+        introduce forall lt (fs_r:fs_val (qResexn qFileDescr)). fs_beh fs_e h lt fs_r ==> exists e'. (qResexn qFileDescr) ∈ (h++lt, fs_r, e') /\ e_beh e e' h lt with begin
+          introduce fs_beh fs_e h lt fs_r ==> exists e'. (qResexn qFileDescr) ∈ (h++lt, fs_r, e') /\ e_beh e e' h lt with _. begin
+            helper_equiv_oprod_openfile_steps h lt fs_fnm' fs_r fnm
+          end
+        end
+      end
+    end
+  end
+#pop-options
 
+#push-options "--split_queries always"
 let equiv_oprod_read #g (fs_fd:fs_oprod g qFileDescr) (fd:exp)
   : Lemma
     (requires fs_fd ⊑ fd)
     (ensures fs_oprod_read fs_fd ⊑ ERead fd)
-  = admit ()
+  =
+  lem_fv_in_env_read g fd;
+  introduce forall b' (s:gsub g b') fsG h. fsG `(≍) h` s ==> (qResexn qString) ⫃ (h, (fs_oprod_read fs_fd) fsG, gsubst s (ERead fd)) with begin
+    introduce _ ==> _ with _. begin
+      let fs_fd' : fs_prod qFileDescr = fs_fd fsG in
+      let fs_e = fs_prod_bind fs_fd' (fun fd' -> read fd') in
+      assert (fs_e == (fs_oprod_read fs_fd) fsG) by (
+        norm [delta_only [`%fs_oprod_read;`%fs_oprod_bind';`%fs_oprod_bind;`%fs_oprod_return_prod]];
+        l_to_r [`lem_hd_stack;`tail_stack_inverse];
+        trefl ());
+      let e = ERead (gsubst s fd) in
+      assert (gsubst s (ERead fd) == e);
+      let ERead fd = e in
+      introduce fsG `(≍) h` s ==> (qResexn qString) ⫃ (h, fs_e, e) with _. begin
+        lem_shift_type_value_environments h fsG s;
+        introduce forall lt (fs_r:fs_val (qResexn qString)). fs_beh fs_e h lt fs_r ==> exists e'. (qResexn qString) ∈ (h++lt, fs_r, e') /\ e_beh e e' h lt with begin
+          introduce fs_beh fs_e h lt fs_r ==> exists e'. (qResexn qString) ∈ (h++lt, fs_r, e') /\ e_beh e e' h lt with _. begin
+            helper_equiv_oprod_read_steps h lt fs_fd' fs_r fd
+          end
+        end
+      end
+    end
+  end
+#pop-options
 
+#push-options "--split_queries always"
 let equiv_oprod_write #g (fs_fd:fs_oprod g qFileDescr) (fs_msg:fs_oprod g qString) (fd msg:exp)
   : Lemma
     (requires fs_fd ⊑ fd /\ fs_msg ⊑ msg)
     (ensures fs_oprod_write fs_fd fs_msg ⊑ EWrite fd msg)
-  = admit ()
+  =
+  lem_fv_in_env_write g fd msg;
+  introduce forall b' (s:gsub g b') fsG h. fsG `(≍) h` s ==> (qResexn qUnit) ⫃ (h, (fs_oprod_write fs_fd fs_msg) fsG, gsubst s (EWrite fd msg)) with begin
+    introduce _ ==> _ with _. begin
+      let fs_fd' : fs_prod qFileDescr = fs_fd fsG in
+      let fs_msg' : fs_prod qString = fs_msg fsG in
+      let fs_e = fs_prod_bind fs_fd' (fun fd' -> fs_prod_bind #qString #(qResexn qUnit) fs_msg' (fun msg' -> write (fd', msg'))) in
+      assert (fs_e == (fs_oprod_write fs_fd fs_msg) fsG) by (
+        norm [delta_only [`%fs_oprod_write;`%fs_oprod_bind';`%fs_oprod_bind;`%fs_oprod_return_prod]];
+        l_to_r [`lem_hd_stack;`tail_stack_inverse];
+        trefl ());
+      let e = EWrite (gsubst s fd) (gsubst s msg) in
+      assert (gsubst s (EWrite fd msg) == e);
+      let EWrite fd msg = e in
+      introduce fsG `(≍) h` s ==> (qResexn qUnit) ⫃ (h, fs_e, e) with _. begin
+        lem_shift_type_value_environments h fsG s;
+        introduce forall lt (fs_r:fs_val (qResexn qUnit)). fs_beh fs_e h lt fs_r ==> exists e'. (qResexn qUnit) ∈ (h++lt, fs_r, e') /\ e_beh e e' h lt with begin
+          introduce fs_beh fs_e h lt fs_r ==> exists e'. (qResexn qUnit) ∈ (h++lt, fs_r, e') /\ e_beh e e' h lt with _. begin
+            helper_equiv_oprod_write_steps h lt fs_fd' fs_msg' fs_r fd msg
+          end
+        end
+      end
+    end
+  end
+#pop-options
 
+#push-options "--split_queries always"
 let equiv_oprod_close #g (fs_fd:fs_oprod g qFileDescr) (fd:exp)
   : Lemma
     (requires fs_fd ⊑ fd)
     (ensures fs_oprod_close fs_fd ⊑ EClose fd)
-  = admit ()
+  =
+  lem_fv_in_env_close g fd;
+  introduce forall b' (s:gsub g b') fsG h. fsG `(≍) h` s ==> (qResexn qUnit) ⫃ (h, (fs_oprod_close fs_fd) fsG, gsubst s (EClose fd)) with begin
+    introduce _ ==> _ with _. begin
+      let fs_fd' : fs_prod qFileDescr = fs_fd fsG in
+      let fs_e = fs_prod_bind fs_fd' (fun fd' -> close fd') in
+      assert (fs_e == (fs_oprod_close fs_fd) fsG) by (
+        norm [delta_only [`%fs_oprod_close;`%fs_oprod_bind';`%fs_oprod_bind;`%fs_oprod_return_prod]];
+        l_to_r [`lem_hd_stack;`tail_stack_inverse];
+        trefl ());
+      let e = EClose (gsubst s fd) in
+      assert (gsubst s (EClose fd) == e);
+      let EClose fd = e in
+      introduce fsG `(≍) h` s ==> (qResexn qUnit) ⫃ (h, fs_e, e) with _. begin
+        lem_shift_type_value_environments h fsG s;
+        introduce forall lt (fs_r:fs_val (qResexn qUnit)). fs_beh fs_e h lt fs_r ==> exists e'. (qResexn qUnit) ∈ (h++lt, fs_r, e') /\ e_beh e e' h lt with begin
+          introduce fs_beh fs_e h lt fs_r ==> exists e'. (qResexn qUnit) ∈ (h++lt, fs_r, e') /\ e_beh e e' h lt with _. begin
+            helper_equiv_oprod_close_steps h lt fs_fd' fs_r fd
+          end
+        end
+      end
+    end
+  end
+#pop-options
